Forgot to commit.

src/Ins.fst
@@ -4,6 +4,8 @@ open Regs
 open State
 open Operand
 open Types
+open FStar.Tactics
+open FStar.Tactics.Typeclasses
 
 (*
 let add64_seman (dst : t1) (src : t2) [|operand nat64 t1|] [|operand nat64 t2|] : st unit =
@@ -16,21 +18,23 @@ let add64_seman (dst : t1) (src : t2) [|operand nat64 t1|] [|operand nat64 t2|] 
 
 type add64 't1 't2 = {
   dst: 't1;
-  src: 't2;
-  dst_operand: operand nat64 't1;
-  src_operand: operand nat64 't2
+  src: 't2
 }
 
-val eval_add64 : add64 't1 't2 -> st unit
-let eval_add64 i =
+(* #set-options "--print_implicits" *)
+let eval_add64 (#t1:Type) (#t2:Type) [|operand nat64 t1|] [|operand nat64 t2|]
+  (i:add64 t1 t2) : st unit =
   s <-- get;
-  let sum = (i.dst_operand.eval_operand i.dst s + i.src_operand.eval_operand i.src s) % pow2_64 in
-  i.dst_operand.update_operand i.dst sum
+  let a : nat64 = eval_operand i.dst s in
+  let b : nat64 = eval_operand i.src s in
+  let sum : nat64 = (a + b) % pow2_64 in
+  update_operand i.dst sum
 
-val add64_to_string : [|show t1, show t2|] -> add64 't1 't2 -> string
-let add64_to_string t = "addf64 "a ^ show t.dst ^ " " ^ show t.src
+val add64_to_string : add64 't1 't2 -> string
+let add64_to_string _ = ""
 
-let add64_ins (#t1:Type)(#t2:Type) : ins (add64 t1 t2) = {
+let add64_ins (#t1:Type)(#t2:Type)[|operand nat64 t1|] [|operand nat64 t2|] :
+  ins (add64 t1 t2) = {
   eval_ins = eval_add64;
   ins_to_string = add64_to_string #t1 #t2
 }
