src/Operand.fsti
@@ -1,6 +1,8 @@
 module Operand
 
 open State
+open FStar.Tactics
+open FStar.Tactics.Typeclasses
 
 noeq type operand 'val 'op = {
   valid_operand     : 'op -> state -> bool;
@@ -9,3 +11,14 @@ noeq type operand 'val 'op = {
   update_operand    : 'op -> 'val -> st unit;
   eval_operand      : 'op -> state -> 'val
 }
+
+[@tcnorm] let valid_operand (#v:Type) (#op:Type) [|op : operand v op |] =
+  op.valid_operand
+[@tcnorm] let valid_dst_operand (#v:Type) (#op:Type) [|op : operand v op |] =
+  op.valid_dst_operand
+[@tcnorm] let check_operand (#v:Type) (#op:Type) [|op : operand v op |] =
+  op.check_operand
+[@tcnorm] let update_operand (#v:Type) (#op:Type) [|op : operand v op |] =
+  op.update_operand
+[@tcnorm] let eval_operand (#v:Type) (#op:Type) [|op : operand v op |] =
+  op.eval_operand
