src/Operand64.fst
@@ -3,10 +3,12 @@ open Regs
 open Operand
 open State
 open Types
+open FStar.Tactics
+open FStar.Tactics.Typeclasses
 
 type const64 = { const: nat64 }
 
-let operandConst64 : operand nat64 const64 = {
+[@instance] let operandConst64 : operand nat64 const64 = {
   valid_operand     = (fun op _  -> 0 <= op.const && op.const < pow2_64 );
   valid_dst_operand = (fun _ -> false);
   check_operand     = (fun _ _  -> true);
@@ -14,7 +16,7 @@ let operandConst64 : operand nat64 const64 = {
   eval_operand      = (fun op _ -> op.const)
 }
 
-let operandReg64 : operand nat64 (regtyp gReg) = {
+[@instance] let operandReg64 : operand nat64 (regtyp gReg) = {
   valid_operand     = (fun _ _  -> true);
   valid_dst_operand = (fun op -> op <> rsp);
   check_operand     = (fun _ _   -> true);
