src/Regs.fst
@@ -3,12 +3,12 @@ module Regs
 open Types
 open FStar.FunctionalExtensionality
 
-let n_reg_t : n:nat{0 < n} = 2
+let n_reg_t : pos = 2
 
 let gReg : reg_t = 0
 let mReg : reg_t = 1
 
-let n_regtype _ : n:nat{0 < n} = 16
+let n_regtype _ : pos = 16
 
 let regval n =
   if n = 0 then nat64 else quad32
